rupicola/stlc/QTyp.fsti
@@ -8,9 +8,7 @@ open STLC
 
 (** We define quotation for Type **)
 
-(** Cezar: why do we need quotation for types?
-      We use it to define the logical relation.
-**)
+(** We need quotation for types to define the logical relation. **)
 noeq
 type type_quotation : Type0 -> Type u#1 =
 | QUnit : type_quotation unit
